hashtable_model.v
@@ -1,0 +1,210 @@
+From stdpp Require Export list fin_maps.
+From iris.program_logic Require Import hoare.
+From iris.heap_lang Require Export lifting notation.
+From iris_hashtable Require Import util.
+
+Class Hashable Σ `{heapG Σ} (Key : Type) `{EqDecision Key} (Hash : Key -> nat) :=
+  { equalf : val;
+    hashf : val;
+    as_key : val -> option Key;
+    
+    equal_spec (k1 k2: Key) (v1 v2: val) :
+      as_key v1 = Some k1 ->
+      as_key v2 = Some k2 ->
+      WP equalf v1 v2 {{u, ⌜u = #(bool_decide (k1 = k2))⌝}}%I;
+      
+    hash_spec k v : as_key v = Some k -> WP hashf v {{u, ⌜u = #(Hash k)⌝}}%I }.
+
+Section model.
+  Context {Σ Key Hash map} `{FinMap Key map, heapG Σ, !Hashable Σ Key Hash}.
+
+  Implicit Type m : map (list val).
+  
+  Definition insert_val m k x := (<[k := x :: from_option id [] (m !! k)]>m).
+  
+  Definition remove_val m k := match m !! k with
+                               | Some (x :: y :: l) => <[k := y :: l]> m
+                               | Some _ => delete k m
+                               | None => m
+                               end.
+
+                                 (*(<[ k := tail (lookup_all M k)]>M).*)
+
+  Definition all_elements m := map_fold (fun k l acc => ((fun v => (k, v)) <$> l) ++ acc) [] m.
+
+  Definition table_wf m := map_Forall (fun _ l => exists x xs, l = x :: xs) m.
+
+  Lemma table_wf_empty : table_wf ∅.
+  Proof. apply map_Forall_empty. Qed.
+  
+  Lemma table_wf_insert_val m k x : table_wf m -> table_wf (insert_val m k x).
+  Proof. apply map_Forall_insert_2. eauto. Qed.
+
+  Lemma table_wf_remove_val m k : table_wf m -> table_wf (remove_val m k).
+  Proof.
+    unfold remove_val.
+    case_eq (m !! k) ; last done.
+    intros [|?[|]] Hlookup ; last (apply map_Forall_insert_2 ; eauto).
+    all: rewrite -{1}(insert_id _ _ _ Hlookup) -insert_delete ;
+      apply map_Forall_insert_12, lookup_delete.
+  Qed.
+
+  Definition lookup_insert_val_ne m k k' x :
+    k ≠ k' -> (insert_val m k x) !! k' = m !! k'. 
+  Proof.
+    intros Hne. rewrite /insert_val lookup_insert_ne //.
+  Qed.
+  
+  Definition lookup_remove_val_ne m k k' :
+    k ≠ k' -> (remove_val m k) !! k' = m !! k'. 
+  Proof.
+    intros Hne. unfold remove_val.
+    case_eq (m !! k) ; last done.
+    intros [|?[|]] Hlookup ; [apply lookup_delete_ne ..| apply lookup_insert_ne] ; done.
+  Qed.
+  
+  Inductive removal : map (list val) -> list (val * val) -> map (list val) -> Prop :=
+  | RemovalNil {m} : removal m [] m
+  | RemovalCons {k k' x xs l m m' } :
+      as_key k = Some k' ->
+      m !! k' = Some (x :: xs) ->
+      removal (remove_val m k') l m' ->
+      removal m ((k, x) :: l) m'.   
+    
+  Lemma removal_app_1 m seq m' seq' m'':
+    removal m seq m' ->
+    removal m' seq' m'' ->
+    removal m (seq ++ seq') m''.
+  Proof.
+    intro HRem. induction HRem as [|] ; [done | econstructor ; eauto].
+  Qed.
+  
+  Lemma removal_app_2 m m' seq seq' :
+    removal m (seq ++ seq') m' ->
+    exists m'', removal m seq m'' /\ removal m'' seq' m'. 
+  Proof.
+    revert m.
+    induction seq as [|[k x] seq IH].
+    - simpl. intros m ?. exists m. split. by constructor 1. assumption.
+    - simpl. intros m Hrem. inversion Hrem as [| ? k' ??????? Hrem']. simplify_eq.
+      specialize (IH (remove_val m k') Hrem'). destruct IH as [m'' [Hseq Hseq']].
+      exists m''. split.
+      by econstructor. assumption.
+  Qed.
+  
+  Definition permitted m seq := exists m', removal m seq m'.
+  Definition complete m seq := removal m seq ∅ .
+
+  Lemma complete_all_elements m seq:
+    complete m seq ->
+    exists seq', Forall2 (fun '(k, x) '(k', x') => x = x' /\ as_key k' = Some k) seq' seq /\
+                 seq' ≡ₚ all_elements m.
+  Proof.
+    assert (forall (k : Key) (l : list val),
+               Proper (Permutation ==> Permutation) (fun acc => ((fun x => (k, x)) <$> l) ++ acc)).
+    { solve_proper. }
+    assert ( forall A (l1 l2 l3 : list A),
+               l1 ++ l2 ++ l3 ≡ₚ l2 ++ l1 ++ l3).
+    { intros. do 2 rewrite app_assoc. f_equiv. apply Permutation_app_comm. }
+    revert m. induction seq as [|[k x] seq IH].
+    - intros m HCom. exists [].
+      split ; first done. inversion HCom.
+       by rewrite  /all_elements map_fold_empty.
+    - intros m HCom. inversion HCom as [| ??k'?????? Hlookup HRem].
+      specialize (IH _ HRem). destruct IH as [seq' [Hforall HPerm]].
+      exists ((k', x) :: seq'). split.
+      + by apply Forall2_cons.
+      + rewrite HPerm /all_elements /remove_val Hlookup. destruct xs.
+        * rewrite -{2}(insert_id m k' [x]) // -insert_delete.
+          rewrite (map_fold_insert Permutation) //. apply lookup_delete.
+        * rewrite -insert_delete (map_fold_insert Permutation) // ; last apply lookup_delete.
+          rewrite app_comm_cons  -fmap_cons.
+          rewrite -{2}(insert_id m k' (x :: v :: xs)) // -insert_delete.
+          rewrite (map_fold_insert Permutation) //. apply lookup_delete.
+  Qed.
+      
+End model.
+
+Structure table Σ key hash map `{FinMap key map, heapG Σ, !Hashable Σ key hash} : Type :=
+  { table_create : val ;
+    table_insert : val ;
+    table_remove : val ;
+    table_lookup : val ;
+    table_fold : val ;
+    table_cascade : val ;
+
+    table_state : Type ;
+    table_in_state : map (list val) -> table_state -> val -> iProp Σ ;
+    is_cascade : map (list val) -> val -> list (val * val) -> table_state -> val -> iProp Σ ;
+
+    table_in_state_wf m state t : (table_in_state m state t → ⌜table_wf m⌝)%I ;
+    is_cascade_persistent m f seq state t : PersistentP (is_cascade m f seq state t) ;
+    
+    table_create_spec (n : nat) : (n > 0)%nat -> WP table_create #n {{t, ∃ state, table_in_state ∅ state t}}%I ;
+    
+    table_insert_spec (t k x : val) m state k' :
+      as_key k = Some k' ->
+      {{{table_in_state m state t}}}
+        table_insert t k x
+        {{{state', RET #(); table_in_state (insert_val m k' x) state' t}}} ;
+
+    table_remove_spec m state t k k' :
+      as_key k = Some k' ->
+      {{{table_in_state m state t}}}
+        table_remove t k
+      {{{ state', RET match m !! k' with
+                      | Some (v :: _) => SOMEV v
+                      | _ => NONEV end ;
+          table_in_state (remove_val m k') state' t }}} ;
+
+    table_lookup_spec m state t k k' :
+      as_key k = Some k' ->
+      {{{table_in_state m state t}}}
+        table_lookup t k
+        {{{ RET match m !! k' with
+                | Some (v :: _) => SOMEV v
+                | _ => NONEV end ;
+            table_in_state m state t }}} ;
+    
+    table_fold_spec m state I (f t a : val) :
+      ((∀ k x seq (a' : val),
+           ⌜permitted m (seq ++ [(k,x)])⌝ →
+           {{I seq a'}} f k x a' {{v, I (seq ++ [(k,x)]) v }}) →
+       {{{table_in_state m state t ∗ I [] a}}}
+         table_fold f t a
+       {{{v seq, RET v; ⌜complete m seq⌝ ∗ table_in_state m state t ∗ I seq v}}})%I ;
+
+    is_cascade_spec m f seq state t:
+      {{{ is_cascade m f seq state t ∗ table_in_state m state t }}}
+        f #()
+      {{{v k x f' , RET v; table_in_state m state t ∗
+                           ((⌜v = NONEV⌝ ∗ ⌜complete m seq⌝) ∨
+                            (⌜v = SOMEV ((k, x), f')⌝ ∗
+                             ⌜permitted m (seq ++ [(k, x)])⌝ ∗           
+                             is_cascade m f' (seq ++ [(k, x)]) state t)) }}};
+
+    table_cascade_spec m state t:
+      {{{table_in_state m state t}}}
+        table_cascade t
+        {{{f, RET f; is_cascade m f [] state t ∗ table_in_state m state t }}}
+  }.
+Arguments table_create {_ _ _ _ _ _ _ _ _ _ _ _ _ _ _} _.
+Arguments table_insert {_ _ _ _ _ _ _ _ _ _ _ _ _ _ _} _.
+Arguments table_remove {_ _ _ _ _ _ _ _ _ _ _ _ _ _ _} _.
+Arguments table_lookup {_ _ _ _ _ _ _ _ _ _ _ _ _ _ _} _.
+Arguments table_fold {_ _ _ _ _ _ _ _ _ _ _ _ _ _ _} _.
+Arguments table_cascade {_ _ _ _ _ _ _ _ _ _ _ _ _ _ _} _.
+Arguments table_state {_ _ _ _ _ _ _ _ _ _ _ _ _ _ _} _.
+Arguments table_in_state {_ _ _ _ _ _ _ _ _ _ _ _ _ _ _} _ _ _ _.
+Arguments is_cascade {_ _ _ _ _ _ _ _ _ _ _ _ _ _ _} _ _ _ _ _ _.
+Arguments table_in_state_wf {_ _ _ _ _ _ _ _ _ _ _ _ _ _ _} _ _ _ _.
+Arguments is_cascade_persistent {_ _ _ _ _ _ _ _ _ _ _ _ _ _ _} _ _ _ _ _ _.
+Arguments table_create_spec {_ _ _ _ _ _ _ _ _ _ _ _ _ _ _} _ _ _.
+Arguments table_insert_spec {_ _ _ _ _ _ _ _ _ _ _ _ _ _ _} _ _ _ _ _ _ _ _ _.
+Arguments table_remove_spec {_ _ _ _ _ _ _ _ _ _ _ _ _ _ _} _ _ _ _ _ _ _ _.
+Arguments table_lookup_spec {_ _ _ _ _ _ _ _ _ _ _ _ _ _ _} _ _ _ _ _ _ _ _.
+Arguments table_fold_spec {_ _ _ _ _ _ _ _ _ _ _ _ _ _ _} _ _ _ _ _ _ _.
+Arguments is_cascade_spec {_ _ _ _ _ _ _ _ _ _ _ _ _ _ _} _ _ _ _ _ _ _.
+Arguments table_cascade_spec {_ _ _ _ _ _ _ _ _ _ _ _ _ _ _} _ _ _ _ _.
+
+Existing Instance is_cascade_persistent.
