partial_table_specs.v
@@ -1,0 +1,116 @@
+From stdpp Require Import bset.
+From iris.proofmode Require Import tactics.
+From iris.algebra Require Import auth.
+From iris.program_logic Require Import hoare.
+From iris.heap_lang.lib Require Import lock.
+From iris_hashtable Require Import array hashtable_conc partial_table util.
+
+Instance partial_table_auth_discrete M K `{FinMap K M} V : CMRADiscrete (authR (partial_tableUR K V M)).
+Proof. apply _. Qed.
+Class partialG M K `{FinMap K M} V Σ := {partial_inG :> inG Σ (authR (partial_tableUR K V M))}.
+Section derived.
+  Context map key Σ hash `{FinMap key map} `{!heapG Σ} `{!Hashable Σ key hash} `{!Array Σ} `{!partialG map key val Σ}.
+  Variable lck : lock Σ.
+  Definition partial_inv γ m : iProp Σ := own γ (● PTCar (m, ⊤)).
+  Definition partial_own γ m d : iProp Σ := own γ (◯ PTCar (m, d)).
+
+  Lemma own_partial_table_lookup γ m m' d k :
+    k ∈ d ->
+    (partial_inv γ m ∗ partial_own γ m' d → ⌜m !! k = m' !! k⌝)%I.
+  Proof.
+    intro Hin. rewrite -own_op. iIntros "Hown".
+    iDestruct (own_valid with "Hown") as "Hval". rewrite uPred.discrete_valid.
+    iDestruct "Hval" as "%". rename_last Hval. iPureIntro.
+    rewrite -(lookup_cut_table_elem_of m d) // -(partial_table_included_cut_table m' _ _ ⊤) //.
+    split. apply multiset_top_no_dup. eauto.
+    apply auth_valid_discrete_2 in Hval. by destruct Hval.
+  Qed.
+
+  Lemma partial_table_create_spec N (n : nat):
+    n > 0 ->
+    WP create_table Σ lck #n
+       {{t, ∃ γ, is_table Σ key hash map lck N (partial_inv γ) t ∗ partial_own γ ∅ ⊤}}%I.
+  Proof.
+    intro. iMod (own_alloc (● PTCar (∅, ⊤) ⋅ ◯ PTCar (∅, ⊤))) as (γ) "[Hinv Hown]".
+    apply auth_valid_discrete_2. split. done. split. apply multiset_top_no_dup. done.
+    iApply (create_table_spec _ _ _ _ _ _ (partial_inv γ) with "Hinv"). done.
+    iNext. iIntros. iExists (γ). iFrame "#". iFrame.
+  Qed.
+  
+  Lemma partial_table_insert_spec N γ m d k k' x t:
+    as_key k' = Some k ->
+    k ∈ d ->
+    {{{is_table Σ key hash map lck N (partial_inv γ) t ∗ partial_own γ m d }}}
+      (table_insert Σ key hash lck) t k' x
+    {{{RET #(); partial_own γ (insert_val m k x) d}}}.
+  Proof.
+    intros Hkey Hin. iIntros (Φ) "[#Htable Hown] HΦ".
+    iApply (table_insert_spec with "[$Htable Hown]") ; try done.
+    iIntros (m') "Hinv". unfold insert_val.
+    iDestruct (own_partial_table_lookup with "[$Hown $Hinv]") as "%". done.
+    rename_last Heq. rewrite Heq.
+    iApply own_op. iApply bupd_fupd. iApply own_update.
+    apply auth_update, partial_table_local_update_partial_alter. done.
+    iSplitL "Hinv" ; iFrame.
+  Qed.
+
+  Lemma partial_table_lookup_spec N γ m d k k' t:
+    as_key k' = Some k ->
+    k ∈ d ->
+    {{{is_table Σ key hash map lck N (partial_inv γ) t ∗ partial_own γ m d }}}
+      (table_lookup Σ key hash) t k'
+    {{{RET match m !! k with
+             Some (v :: _) => SOMEV v
+           | _ => NONEV end ;
+       partial_own γ m d}}}.
+  Proof.
+    intros Hkey Hin. iIntros (Φ) "[#Htable Hown] HΦ".
+    iApply (table_lookup_spec _ _ _ _ _ _ _
+                              (fun _ x => (∃ xs, ⌜m !! k = Some (x :: xs)⌝) ∗ partial_own γ m d)%I
+                              (⌜m !! k = None⌝ ∗ partial_own γ m d)%I
+              with "[$Htable Hown]") ; try done.
+    iSplit ; [iIntros (m' Hlookup) | iIntros (m' x xs Hlookup)] ; iIntros "Hinv !>" ;
+      iDestruct (own_partial_table_lookup with "[$Hown $Hinv]") as "%" ; try done ;
+      rename_last Heq ; rewrite Heq in Hlookup ; iFrame ; eauto.
+    iNext.
+    iIntros (? ?) "[[% [% ?]]|[% [Hex ?]]]" ; last iDestruct "Hex" as (?) "%" ;
+      simplify_eq ; rename_last Hlookup ; rewrite Hlookup ;
+      iApply "HΦ" ; iFrame.
+  Qed.
+
+  Lemma partial_table_remove_spec N γ m d k k' t:
+    as_key k' = Some k ->
+    k ∈ d ->
+    {{{is_table Σ key hash map lck N (partial_inv γ) t ∗ partial_own γ m d }}}
+      (table_remove Σ key hash lck) t k'
+    {{{RET match m !! k with
+             Some (v :: _) => SOMEV v
+           | _ => NONEV end ;
+       partial_own γ (remove_val m k) d}}}.
+  Proof.
+    intros Hkey Hin. iIntros (Φ) "[#Htable Hown] HΦ".
+    iApply (table_remove_spec _ _ _ _ _ _ _
+                               (fun _ x =>
+                                  (∃ xs, ⌜m !! k = Some (x :: xs)⌝) ∗
+                                  partial_own γ (remove_val m k) d)%I
+                               (⌜m !! k = None⌝ ∗
+                                 partial_own γ m d)%I
+              with "[$Htable Hown]") ; try done.
+    {
+      iSplit ; [iIntros (m' Hlookup) | iIntros (m' ? x Hlookup) ] ; iIntros "Hinv" ;
+        iDestruct (own_partial_table_lookup with "[$Hown $Hinv]") as "%";
+        try done ; rename_last Heq ; rewrite Heq in Hlookup.
+      - iFrame. done.
+      - rewrite [(_ ∗ partial_own _ _ _)%I]comm assoc. iSplitL ; last eauto.
+        iApply own_op. iApply bupd_fupd. iApply own_update.
+        rewrite /remove_val Heq Hlookup.
+        apply auth_update. destruct x ; by apply partial_table_local_update_partial_alter.
+        iApply own_op. iFrame.
+    }
+    iNext.
+    iIntros (? ?) "[[% [% ?]]|[% [% ?]]]" ; simplify_eq ;
+      rename_last Hlookup ; last destruct Hlookup as [? Hlookup] ;
+      rewrite /remove_val Hlookup ; iApply "HΦ" ; iFrame.
+  Qed.
+  
+End derived.
